no need for lift_store; finish LogRel

steel/Zeta.Steel.LogRel.fst
@@ -1,12 +1,65 @@
 module Zeta.Steel.LogRel
 
+module GV = Zeta.GenericVerifier
+
+let rec map_ghost (p:'a -> Type0) 
+                  (s:Seq.seq 'a { forall (i:Zeta.SeqAux.seq_index s). p (Seq.index s i) })
+                  (f: (x:'a { p x } -> GTot 'b))
+  : GTot (s':Seq.seq 'b { Seq.length s == Seq.length s' /\
+                         (forall (i:Zeta.SeqAux.seq_index s). Seq.index s' i == f (Seq.index s i)) })
+         (decreases (Seq.length s))
+  = if Seq.length s = 0 then Seq.empty
+    else (
+      let prefix, last = Seq.un_snoc s in
+      Seq.snoc (map_ghost p prefix f) (f last)
+    )
+                           
+let lift_slots (s:Seq.seq s_slot_id { forall (i:Zeta.SeqAux.seq_index s). valid_slot (Seq.index s i)  })
+  : GTot (is:Seq.seq i_slot_id  { Seq.length s = Seq.length is /\
+                                  (forall i. related_slot (Seq.index s i) (Seq.index is i)) })
+         (decreases (Seq.length s))
+  = map_ghost (fun x -> valid_slot x) s lift_slot
+  
 let lift_log_entry (se: s_log_entry {valid_log_entry se})
-  : ie: i_log_entry { related_log_entry se ie }
-  = admit()
+  : GTot (ie: i_log_entry { related_log_entry se ie })
+  = let open Zeta.Steel.LogEntry.Types in
+    let open Zeta.Steel.Rel in
+    match se with
+    | AddM s s' r ->
+      let i_r = lift_record r in
+      let i_s = lift_slot s in
+      let i_s' = lift_slot s' in
+      GV.AddM i_r i_s i_s'
+
+    | AddB s t tid r ->
+      let i_r = lift_record r in
+      let i_s = lift_slot s in
+      let i_t = lift_timestamp t in
+      let i_tid = lift_tid tid in
+      GV.AddB i_r i_s i_t i_tid
+
+    | EvictM p ->
+      GV.EvictM (lift_slot p.s) (lift_slot p.s_)
+
+    
+    | EvictB p ->
+      GV.EvictB (lift_slot p.s) (lift_timestamp p.t)
+
+    | EvictBM p ->
+      GV.EvictBM (lift_slot p.s) (lift_slot p.s_) (lift_timestamp p.t)
+
+    | NextEpoch ->
+      GV.NextEpoch
+
+    | VerifyEpoch ->
+      GV.VerifyEpoch
+
+    | RunApp p ->
+      GV.RunApp p.fid (parse_arg p.fid p.rest) (lift_slots (parse_slots p.fid p.rest))
 
 let lift_log (sl: s_log {valid_log sl})
-  : il:i_log {related_log sl il}
-  = admit()
+  : GTot (il:i_log {related_log sl il})
+  = map_ghost valid_log_entry sl lift_log_entry
 
 let lift_log_snoc (sl: s_log {valid_log sl}) (se: s_log_entry {valid_log_entry se})
   : Lemma (requires (let sl_ = Seq.snoc sl se in
@@ -18,13 +71,15 @@ let lift_log_snoc (sl: s_log {valid_log sl}) (se: s_log_entry {valid_log_entry s
                     let i = Seq.length sl in
                     il_ == Seq.snoc il ie /\
                     Seq.index il_ i = ie))
-  = admit()
+  = let sl_ = Seq.snoc sl se in
+    let prefix, last = Seq.un_snoc sl_ in
+    assert (prefix `Seq.equal` sl)
 
 let prefix_of_valid_valid (l: s_log {valid_log l}) (i: nat{ i <= Seq.length l})
   : Lemma (ensures (let l' = SA.prefix l i in
                     valid_log l'))
-  = admit()
+  = ()
 
 let lift_prefix_commute (l: s_log {valid_log l}) (i: nat{ i <= Seq.length l})
   : Lemma (ensures (lift_log (SA.prefix l i) == SA.prefix (lift_log l) i))
-  = admit()
+  = assert (lift_log (SA.prefix l i) `Seq.equal` SA.prefix (lift_log l) i)
