steel/Zeta.Steel.StoreRel.fst
@@ -5,43 +5,6 @@ open FStar.Classical
 module IS = Zeta.Intermediate.Store
 module TSM = Zeta.Steel.ThreadStateModel
 
-let lift_store_entry (s: s_store_entry)
-  : GTot (i:i_store_entry { related_store_entry s i })
-  = let open Zeta.High.Verifier in
-    let r = lift_record (s.key, s.value) in
-    let am = 
-      match s.add_method with
-      | TSM.MAdd -> MAdd
-      | TSM.BAdd -> BAdd
-    in
-    let ld =
-      match s.l_child_in_store with
-      | None -> None
-      | Some s -> Some (lift_slot s)
-    in
-    let rd =
-      match s.r_child_in_store with
-      | None -> None
-      | Some s -> Some (lift_slot s)
-    in    
-    let p =
-      match s.parent_slot with
-      | None -> None
-      | Some (s,d) ->
-        Some (lift_slot s, 
-              (if d then Zeta.BinTree.Left else Zeta.BinTree.Right))
-    in
-    Zeta.Intermediate.Store.VStoreE r am ld rd p
-
-let lift_store_entries (ss: Seq.seq (option s_store_entry))
-  : GTot (is: Seq.seq (option i_store_entry) { Seq.length ss == Seq.length is /\
-                                               (forall i. Seq.index ss i `related_store_entry_opt` Seq.index is i) })
-  = admit()
-
-let lift_store (ss: s_store)
-  : GTot (is: i_store { related_store ss is })
-  = admit()
-
 #push-options "--fuel 1 --ifuel 1 --query_stats"
 
 let lemma_related_implies_parent_props (st: s_store) (i_st: i_store)
